bilby wordarray: Changed some wordarray axioms to lemmas
Changed several axioms about word arrays, which are used in BilbyFS
proofs, to be lemmas instead. These axioms were for the word array
methods of length, get, map_no_break and for the abstraction functions.

The abstraction functions were changed so that they only worked for
lists and word arrays, whose elements were words. In addition,
constraints were added so that the length of the word array is bounded
by 2 ^ 32, due to that being the maximum length that a word array can be
represented with the current word array implementation.

impl/fs/bilby/proof/adt/WordArrayT.thy
@@ -12,10 +12,16 @@ theory WordArrayT
 imports
   "../adt/BilbyT"
   "../lib/Loops"
+  "../adt/WordArray_Shallow"
 begin
 
-consts \<alpha>wa :: "'a WordArray \<Rightarrow> 'a list"
-consts make :: "'a list \<Rightarrow> 'a WordArray"
+definition \<alpha>wa :: "(('a::len0) word) WordArray \<Rightarrow> ('a word) list"
+  where
+"\<alpha>wa wa = wa"
+
+definition make :: "(('a::len0) word) list \<Rightarrow> ('a word) WordArray"
+  where
+"make xs = xs"
 
 definition
   mapAccumObs :: "nat \<Rightarrow> nat \<Rightarrow> (('a, 'acc, 'obsv) ElemAO \<Rightarrow> ('a \<times> 'acc))
@@ -25,7 +31,7 @@ where
    (let (ys, acc) = fold (\<lambda>elem (ys,acc).
            let (elem,acc) = fn (ElemAO.make elem acc obs)
             in  (ys@[elem], acc)) (slice frm to xs) ([],vacc)
-     in (take frm xs @ ys @ drop (max frm to) xs, acc))"
+     in (take frm xs @ ys @ List.drop (max frm to) xs, acc))"
 
 lemma length_mapAccum_helper:
   "length (fst $ fold (\<lambda>x (ys,a'). let  (elem, acc) = loopbody x a'
@@ -57,7 +63,7 @@ lemma slice_length:
 lemma length_mapAccum_slice_helper':
   "length (take frm xs @ fst (let (xs', acc) = fold (\<lambda>x (ys,a'). let  (elem, acc) = loopbody x a'
                                   in  (ys@[elem],acc)) (slice frm to xs) (ys,a)
-           in (xs',acc))  @ drop (max frm to) xs) = length ys + length xs"
+           in (xs',acc))  @ List.drop (max frm to) xs) = length ys + length xs"
   unfolding Let_def  prod.case_eq_if
   using length_mapAccum_slice_helper[unfolded prod.case_eq_if Let_def, where xs=xs and ys=ys and frm=frm and to=to and loopbody=loopbody and a=a]
   by (simp add: slice_length)
@@ -70,33 +76,74 @@ lemma length_mapAccum:
 
 
 lemma length_mapAccumI:
-  " P (length xs) \<Longrightarrow> P (length (fst (mapAccumObs frm to fn xs a obs)))"
- by (simp add : length_mapAccum)
+  "P (length xs) \<Longrightarrow> P (length (fst (mapAccumObs frm to fn xs a obs)))"
+  by (simp add : length_mapAccum)
+
+lemma wordarray_make:
+  "\<And>xs. \<alpha>wa (WordArrayT.make xs) = xs"
+  by (simp add: \<alpha>wa_def WordArrayT.make_def)
+
+lemma wordarray_make':
+  "\<And>wa. WordArrayT.make (\<alpha>wa wa) = wa"
+  by (simp add: \<alpha>wa_def WordArrayT.make_def)
+
+lemma wordarray_get_ret:
+  "\<lbrakk> unat index < length (\<alpha>wa arr) \<rbrakk> \<Longrightarrow>
+    wordarray_get (arr, index) = \<alpha>wa arr ! unat index"
+  by (simp add: wordarray_get' \<alpha>wa_def)
+
+lemma mapAccum_fold_helper:
+  "fold (\<lambda>a (ys, b). case f (ElemAO.make a b obs) of (a', b') \<Rightarrow> (ys @ [a'], b')) xs ([], acc)
+    = mapAccum (\<lambda>a b. f (ElemAO.make a b obs)) xs acc"
+  apply (induct arbitrary: acc rule: rev_induct)
+   apply clarsimp
+  apply (clarsimp simp: mapAccum_step split: prod.splits)
+  done
+
+lemma wordarray_map_no_break_ret:
+  "\<And>P. (let (aarr, vacc) = mapAccumObs (unat frm) (unat to) body (\<alpha>wa arr) acc obs
+          in P ((WordArrayT.make aarr), vacc)) 
+   \<Longrightarrow> P (wordarray_map_no_break (ArrayMapP.make arr frm to body acc obs))"
+  apply (unfold mapAccumObs_def wordarray_map_no_break')
+  apply clarsimp
+  apply (clarsimp split: prod.splits)
+  apply (rename_tac vacc xs xs' vacc')
+  apply (rule conjI; clarsimp simp: ArrayMapP.make_def \<alpha>wa_def WordArrayT.make_def)
+  apply (clarsimp simp: mapAccum_fold_helper word_le_nat_alt max_def)
+  apply (clarsimp simp: slice_def not_le word_less_nat_alt max_def)
+  done
 
 axiomatization
 where
-  wordarray_make: "\<And>xs. \<alpha>wa (WordArrayT.make xs) = xs"
+(*  wordarray_make: "\<And>xs. \<alpha>wa (WordArrayT.make xs) = xs"
  and
   wordarray_make': "\<And>wa. WordArrayT.make (\<alpha>wa wa) = wa"
- and
-  wordarray_create_ret:
+ and*)
+\<comment> \<open> We need to add that the maximum length of a word array is less than the maximum 32-bit word
+    since wordarray_length returns a 32-bit word.\<close>
+  wordarray_length_max: 
+    "\<And>wa. length (\<alpha>wa wa) \<le> unat (max_word :: 32 word)"
+  and wordarray_length_max': 
+    "\<And>xs. wordarray_length (WordArrayT.make xs) \<le> (max_word :: 32 word)"
+  and wordarray_create_ret:
    "\<And>P.\<lbrakk>  \<And>ex'. (ex', Option.None ()) = malloc ex \<Longrightarrow> P (Error ex');
            \<And>ex' v. \<lbrakk> sz > 0 ; (ex', Option.Some v) = malloc ex; length (\<alpha>wa v) = unat sz \<rbrakk> \<Longrightarrow>
                  P (Success (ex', v))
         \<rbrakk> \<Longrightarrow>
       P (wordarray_create (ex, sz))"
-
+(*
    and wordarray_length_ret:
    "unat (wordarray_length arr) = length (\<alpha>wa arr)"
-
+*)
+(*
   and wordarray_get_ret:
   "\<lbrakk> unat index < length (\<alpha>wa arr) \<rbrakk> \<Longrightarrow>
     wordarray_get (arr, index) = \<alpha>wa arr ! unat index"
-
+*)
   and wordarray_modify_ret:
    "\<And>P. \<lbrakk> unat index < List.length (\<alpha>wa varr);
        let r = modifier (ElemAO.make ((\<alpha>wa varr)!unat index) vacc obs) in
-       P (ArrA.make (WordArrayT.make (\<alpha>wa varr[unat index:=ElemA.elem\<^sub>f r])) (ElemA.acc\<^sub>f r)) \<rbrakk> \<Longrightarrow>
+       P (ArrA.make (WordArrayT.make ((\<alpha>wa varr)[(unat index) := (ElemA.elem\<^sub>f r)])) (ElemA.acc\<^sub>f r)) \<rbrakk> \<Longrightarrow>
         P (wordarray_modify (ArrayUseValueP.make varr index modifier vacc obs))"
 (* Alternative that does not use WordArray.make
   and wordarray_modify_ret:
@@ -105,26 +152,39 @@ where
        \<And>arr'. \<alpha>wa arr' = (\<alpha>wa varr)[unat index:=a] \<Longrightarrow> P (ArrA.make arr' acc'') \<rbrakk> \<Longrightarrow>
         P (wordarray_modify (ArrayUseValueP.make varr index modifier vacc obs))"
 *)
+(*
    and wordarray_map_no_break_ret:
    "\<And>P. (let (aarr, vacc) = mapAccumObs (unat frm) (unat to) body (\<alpha>wa arr) acc obs
           in P ((WordArrayT.make aarr), vacc)) 
    \<Longrightarrow> P (wordarray_map_no_break (ArrayMapP.make arr frm to body acc obs))"
+*)
   and wordarray_cmp_ret:
   "\<And>P. P(\<alpha>wa a1 = \<alpha>wa a2) \<Longrightarrow> P (wordarray_cmp(a1, a2))"
   and wordarray_set_ret:
   "(offs::U32) \<le> offs + len \<Longrightarrow>
    wordarray_set (wa, offs, len, (v::U8)) =
    WordArrayT.make ((take (unat offs) (\<alpha>wa wa) @
-                   replicate (unat len) v @ drop (unat (offs + len)) (\<alpha>wa wa)))"
+                   replicate (unat len) v @ List.drop (unat (offs + len)) (\<alpha>wa wa)))"
 
   and wordarray_copy_ret:
   "\<And>P. \<lbrakk>  length (\<alpha>wa dst) = length (\<alpha>wa src) \<Longrightarrow>
                   offs = src_offs \<Longrightarrow>
                   offs \<le> offs + len \<Longrightarrow>
                   unat (offs + len) \<le> length (\<alpha>wa src) \<Longrightarrow>
-         P (WordArrayT.make (take (unat offs) (\<alpha>wa dst) @ slice (unat offs) (unat offs + unat len) (\<alpha>wa src) @ drop (unat (offs+len)) (\<alpha>wa dst))) \<rbrakk>
+         P (WordArrayT.make (take (unat offs) (\<alpha>wa dst) @ slice (unat offs) (unat offs + unat len) (\<alpha>wa src) @ List.drop (unat (offs+len)) (\<alpha>wa dst))) \<rbrakk>
      \<Longrightarrow>
       P (wordarray_copy(dst, src, offs, src_offs, len))"
+
+
+lemma wordarray_length_ret:
+  "unat (wordarray_length arr) = length (\<alpha>wa arr)"
+  apply (insert wordarray_length_max)
+  apply (drule_tac x = arr in meta_spec)
+  apply (clarsimp simp: wordarray_length' \<alpha>wa_def)
+  apply (rule unat_of_nat_eq)
+  apply (clarsimp simp: max_word_def)
+  done
+
 
 lemma wordarray_\<alpha>wa_eq:
   "\<And>xs ys. (xs = ys) \<longleftrightarrow> \<alpha>wa xs = \<alpha>wa ys"
